<?xml version="1.0"?>
<rdf:RDF xmlns="https://w3id.org/netbeheer/referentiemodellen/gas/Gridmanagement/core#"
     xml:base="https://w3id.org/netbeheer/referentiemodellen/gas/Gridmanagement/core"
     xmlns:owl="http://www.w3.org/2002/07/owl#"
     xmlns:rdf="http://www.w3.org/1999/02/22-rdf-syntax-ns#"
     xmlns:xml="http://www.w3.org/XML/1998/namespace"
     xmlns:xsd="http://www.w3.org/2001/XMLSchema#"
     xmlns:obda="https://w3id.org/obda/vocabulary#"
     xmlns:rdfs="http://www.w3.org/2000/01/rdf-schema#"
     xmlns:terms="http://purl.org/dc/terms/">
    <owl:Ontology rdf:about="https://w3id.org/netbeheer/referentiemodellen/gas/Gridmanagement/core">
        <owl:imports rdf:resource="https://w3id.org/netbeheer/def/TC57CIM/IEC61970/Base/Core"/>
    </owl:Ontology>
    


    <!-- 
    ///////////////////////////////////////////////////////////////////////////////////////
    //
    // Object Properties
    //
    ///////////////////////////////////////////////////////////////////////////////////////
     -->

    


    <!-- https://w3id.org/netbeheer/referentiemodellen/gas/Gridmanagement/core#3cf525a5_236b_4bca_a13c_3d7b1dcf3e1a -->

    <owl:ObjectProperty rdf:about="https://w3id.org/netbeheer/referentiemodellen/gas/Gridmanagement/core#3cf525a5_236b_4bca_a13c_3d7b1dcf3e1a">
        <rdfs:domain rdf:resource="https://w3id.org/netbeheer/referentiemodellen/gas/Gridmanagement/core#213c36e8_224a_44ba_93a6_7f8ce7aae930"/>
        <rdfs:range rdf:resource="https://w3id.org/netbeheer/referentiemodellen/IECCIM/TC57CIM/IEC61970/Base/Core#Terminal"/>
        <rdfs:label xml:lang="nl">HeeftTerminal</rdfs:label>
    </owl:ObjectProperty>
    


    <!-- 
    ///////////////////////////////////////////////////////////////////////////////////////
    //
    // Classes
    //
    ///////////////////////////////////////////////////////////////////////////////////////
     -->

    


    <!-- https://w3id.org/netbeheer/referentiemodellen/IECCIM/TC57CIM/IEC61970/Base/Core#Equipment -->

    <owl:Class rdf:about="https://w3id.org/netbeheer/referentiemodellen/IECCIM/TC57CIM/IEC61970/Base/Core#Equipment"/>
    


    <!-- https://w3id.org/netbeheer/referentiemodellen/IECCIM/TC57CIM/IEC61970/Base/Core#EquipmentContainer -->

    <owl:Class rdf:about="https://w3id.org/netbeheer/referentiemodellen/IECCIM/TC57CIM/IEC61970/Base/Core#EquipmentContainer"/>
    


    <!-- https://w3id.org/netbeheer/referentiemodellen/IECCIM/TC57CIM/IEC61970/Base/Core#IdentifiedObject -->

    <owl:Class rdf:about="https://w3id.org/netbeheer/referentiemodellen/IECCIM/TC57CIM/IEC61970/Base/Core#IdentifiedObject"/>
    


    <!-- https://w3id.org/netbeheer/referentiemodellen/gas/Gridmanagement/core#a03eafa3_2eb3_4656_a7dd_3cba22ef3e56 -->

    <owl:Class rdf:about="https://w3id.org/netbeheer/referentiemodellen/gas/Gridmanagement/core#a03eafa3_2eb3_4656_a7dd_3cba22ef3e56">
        <rdfs:subClassOf rdf:resource="https://w3id.org/netbeheer/referentiemodellen/IECCIM/TC57CIM/IEC61970/Base/Core#EquipmentContainer"/>
        <rdfs:label xml:lang="nl">GInstallatie</rdfs:label>
    </owl:Class>
    


    <!-- https://w3id.org/netbeheer/referentiemodellen/gas/Gridmanagement/core#f7f54270_6b8d_45c0_8314_46223a396f09 -->

    <owl:Class rdf:about="https://w3id.org/netbeheer/referentiemodellen/gas/Gridmanagement/core#f7f54270_6b8d_45c0_8314_46223a396f09">
        <rdfs:subClassOf rdf:resource="https://w3id.org/netbeheer/referentiemodellen/IECCIM/TC57CIM/IEC61970/Base/Core#EquipmentContainer"/>
        <rdfs:comment xml:lang="en">A collection of equipment for purposes other than generation or utilization, through which gas in bulk is passed for the purposes of switching or modifying its characteristics.</rdfs:comment>
        <rdfs:label xml:lang="nl">GStationcomplex</rdfs:label>
        <rdfs:label xml:lang="en">Gas Substation</rdfs:label>
    </owl:Class>
    


    <!-- https://w3id.org/netbeheer/referentiemodellen/gas/Gridmanagement/core#213c36e8_224a_44ba_93a6_7f8ce7aae930 -->

    <owl:Class rdf:about="https://w3id.org/netbeheer/referentiemodellen/gas/Gridmanagement/core#213c36e8_224a_44ba_93a6_7f8ce7aae930">
        <rdfs:subClassOf rdf:resource="https://w3id.org/netbeheer/referentiemodellen/IECCIM/TC57CIM/IEC61970/Base/Core#Equipment"/>
        <rdfs:comment xml:lang="nl">De componenten van het gas systeem dat gas doorlaten ten behoeven van transport en distributie van gas</rdfs:comment>
        <rdfs:comment xml:lang="en">The components of the gas infrastructure that transport or distribute gas. this is the gas equivalent of cim:ConductingEquipment</rdfs:comment>
        <rdfs:label xml:lang="nl">PrimaireComponenten</rdfs:label>
    </owl:Class>
    


    <!-- https://w3id.org/netbeheer/referentiemodellen/gas/Gridmanagement/core#726dcde9_aa71_4891_8e3b_d1b80d8cc7dc -->

    <owl:Class rdf:about="https://w3id.org/netbeheer/referentiemodellen/gas/Gridmanagement/core#726dcde9_aa71_4891_8e3b_d1b80d8cc7dc">
        <rdfs:subClassOf rdf:resource="https://w3id.org/netbeheer/referentiemodellen/IECCIM/TC57CIM/IEC61970/Base/Core#IdentifiedObject"/>
        <rdfs:comment xml:lang="nl">Het classificatie van drukniveau waar het net op berdeven wordt</rdfs:comment>
        <rdfs:comment xml:lang="en">The pressure level at which a section of the grid is operated</rdfs:comment>
        <rdfs:label xml:lang="nl">Drukniveau</rdfs:label>
    </owl:Class>
    


    <!-- https://w3id.org/netbeheer/referentiemodellen/gas/Gridmanagement/core#759e79fd_93c4_4b7f_9df9_e73eabdaac9c -->

    <owl:Class rdf:about="https://w3id.org/netbeheer/referentiemodellen/gas/Gridmanagement/core#759e79fd_93c4_4b7f_9df9_e73eabdaac9c">
        <rdfs:subClassOf rdf:resource="https://w3id.org/netbeheer/referentiemodellen/IECCIM/TC57CIM/IEC61970/Base/Core#EquipmentContainer"/>
        <rdfs:comment xml:lang="en">A section of pipes, regulators, filters, sensors and valves (usually above ground for easy access) used to regulate and transform presure within a Substation.</rdfs:comment>
        <rdfs:label xml:lang="nl">GRegelstraat</rdfs:label>
    </owl:Class>
</rdf:RDF>



<!-- Generated by the OWL API (version 4.5.9.2019-02-01T07:24:44Z) https://github.com/owlcs/owlapi -->

